update to latest riscv-coq, whose load/store primitives get a SourceType
argument telling whether it is from instruction fetch or instruction exec,
and which reorganizes the directory structure.
Refactoring for the updated directory structure was done using

find bedrock2 compiler processor deps/kami -type f -name '*.v' -print0 \
 | xargs -0 sed -i \
  -e 's/riscv\.util\./riscv.Utility./g' \
  -e 's/riscv\.Utility.$/riscv.Utility.Utility./g' \
  -e 's/riscv\.Decode/riscv.Spec.Decode/g' \
  -e 's/riscv\.Program/riscv.Spec.Machine/g' \
  -e 's/riscv\.Memory/riscv.Platform.Memory/g' \
  -e 's/riscv\.Words32Naive/riscv.Utility.Words32Naive/g' \
  -e 's/riscv\.DefaultMemImpl32/riscv.Utility.DefaultMemImpl32/g' \
  -e 's/riscv\.Execute/riscv.Spec.Execute/g' \
  -e 's/riscv\.InstructionCoercions/riscv.Utility.InstructionCoercions/g' \
  -e 's/riscv\.MetricLogging/riscv.Platform.MetricLogging/g' \
  -e 's/riscv\.MetricPrimitives/riscv.Spec.MetricPrimitives/g' \
  -e 's/riscv\.MetricRiscvMachine/riscv.Platform.MetricRiscvMachine/g' \
  -e 's/riscv\.Minimal/riscv.Platform.Minimal/g' \
  -e 's/riscv\.MinimalLogging/riscv.Platform.MinimalLogging/g' \
  -e 's/riscv\.MkMachineWidth/riscv.Utility.MkMachineWidth/g' \
  -e 's/riscv\.MMIOTrace/riscv.Utility.MMIOTrace/g' \
  -e 's/riscv\.Primitives/riscv.Spec.Primitives/g' \
  -e 's/riscv\.RiscvMachine/riscv.Platform.RiscvMachine/g' \
  -e 's/riscv\.Run/riscv.Platform.Run/g' \
  -e 's/riscv\.runsToNonDet/riscv.Utility.runsToNonDet/g' \
  -e 's/riscv\.Encode/riscv.Utility.Encode/g' \
  -e 's/riscv\.InstructionNotations/riscv.Utility.InstructionNotations/g' \
  -e 's/riscv\.proofs\.DecodeEncode/riscv.Proofs.DecodeEncode/g' \
  -e 's/riscv\.proofs\.EncodeBound/riscv.Proofs.EncodeBound/g' \
  -e 's/riscv\.PseudoInstructions/riscv.Spec.PseudoInstructions/g'

compiler/src/EmitsValid.v
@@ -1,18 +1,18 @@
 Require Import Coq.Lists.List. Import ListNotations.
 Require Import Coq.micromega.Lia.
 Require Import Coq.ZArith.ZArith.
-Require Import riscv.Decode.
-Require Import riscv.Encode.
-Require Import riscv.util.ZBitOps.
-Require Import riscv.Run.
-Require Import riscv.Program.
-Require Import riscv.Primitives.
+Require Import riscv.Spec.Decode.
+Require Import riscv.Utility.Encode.
+Require Import riscv.Utility.ZBitOps.
+Require Import riscv.Platform.Run.
+Require Import riscv.Spec.Machine.
+Require Import riscv.Spec.Primitives.
 Require Import compiler.util.Tactics.
-Require Import riscv.util.Tactics.
+Require Import riscv.Utility.Tactics.
 Require Import compiler.FlatImp.
 Require Import compiler.FlatToRiscvDef. Import FlatToRiscvDef.
-Require Import riscv.util.ListLib.
-Require Import riscv.Memory.
+Require Import riscv.Utility.ListLib.
+Require Import riscv.Platform.Memory.
 
 Local Open Scope Z_scope.
 
@@ -262,6 +262,9 @@ Ltac unify_universes_for_lia :=
 (* workaround for https://github.com/coq/coq/issues/9268 *)
 Ltac lia' := unify_universes_for_lia; lia.
 
+Inductive supported_iset: InstructionSet -> Prop :=
+| supported_RV32IM: supported_iset RV32IM
+| supported_RV64IM: supported_iset RV64IM.
 
 Section EmitsValid.
 
@@ -294,7 +297,7 @@ Section EmitsValid.
   Qed.
 
   Lemma compile_op_emits_valid: forall x op y z,
-      supportsM iset = true ->
+      supported_iset iset ->
       valid_register x ->
       valid_register y ->
       valid_register z ->
@@ -304,7 +307,6 @@ Section EmitsValid.
     intros.
     destruct op; simpl in *; (repeat destruct H3; try contradiction);
           inversions H; unfold verify; simpl;
-          unfold supportsM in *;
           autounfold with unf_verify unf_encode_consts;
           unfold Register0;
           repeat match goal with
@@ -338,14 +340,15 @@ Section EmitsValid.
   Qed.
 
   Lemma compile_load_emits_valid: forall x y sz,
+      supported_iset iset ->
       valid_register x ->
       valid_register y ->
       valid_instructions iset [compile_load iset sz x y 0].
   Proof.
     intros.
-    destruct sz; destruct iset eqn: E; unfold valid_instructions, valid_register in *; simpl;
+    destruct sz; inversions H; unfold valid_instructions, valid_register in *; simpl;
       intros;
-      (destruct H1; [|contradiction]);
+      (destruct H; [|contradiction]);
       subst instr;
       unfold verify;
       simpl;
@@ -355,14 +358,15 @@ Section EmitsValid.
   Qed.
 
   Lemma compile_store_emits_valid: forall x y sz,
+      supported_iset iset ->
       valid_register x ->
       valid_register y ->
       valid_instructions iset [compile_store iset sz x y 0].
   Proof.
     intros.
-    destruct sz; destruct iset eqn: E; unfold valid_instructions, valid_register in *; simpl;
+    destruct sz; inversions H; unfold valid_instructions, valid_register in *; simpl;
       intros;
-      (destruct H1; [|contradiction]);
+      (destruct H; [|contradiction]);
       subst instr;
       unfold verify;
       simpl;
@@ -389,7 +393,7 @@ Section EmitsValid.
   Qed.
 
   Lemma compile_stmt_emits_valid: forall s,
-      supportsM iset = true ->
+      supported_iset iset ->
       valid_registers s ->
       stmt_not_too_big s ->
       valid_instructions iset (compile_stmt iset s).
