compiler/src/Basic32Semantics.v
@@ -2,8 +2,8 @@ Require Import Coq.ZArith.ZArith.
 Require Import bedrock2.Syntax bedrock2.Semantics.
 Require Import coqutil.Map.SortedList.
 Require Import bedrock2.ZNamesSyntax.
-Require Import riscv.Words32Naive.
-Require Import riscv.DefaultMemImpl32.
+Require Import riscv.Utility.Words32Naive.
+Require Import riscv.Utility.DefaultMemImpl32.
 Require Import coqutil.Map.Empty_set_keyed_map.
 Require Import coqutil.Map.Z_keyed_SortedListMap.
 
