processor/src/Test.v
@@ -1,26 +1,26 @@
 Require Import Coq.ZArith.ZArith.
 Require Import Coq.micromega.Lia.
 Require Import Coq.Lists.List. Import ListNotations.
-Require Import riscv.Decode.
-Require Import riscv.Encode.
+Require Import riscv.Spec.Decode.
+Require Import riscv.Utility.Encode.
 Require Import coqutil.Word.LittleEndian.
 Require Import coqutil.Word.Properties.
 Require Import coqutil.Map.Interface.
 Require Import coqutil.Tactics.Tactics.
-Require Import riscv.Utility.
-Require Import riscv.Primitives.
-Require Import riscv.RiscvMachine.
-Require Import riscv.Program.
-Require riscv.Memory.
-Require Import riscv.PseudoInstructions.
-Require Import riscv.proofs.EncodeBound.
-Require Import riscv.proofs.DecodeEncode.
-Require Import riscv.Run.
-Require Import riscv.MkMachineWidth.
-Require Import riscv.util.Monads.
-Require Import riscv.runsToNonDet.
+Require Import riscv.Utility.Utility.
+Require Import riscv.Spec.Primitives.
+Require Import riscv.Platform.RiscvMachine.
+Require Import riscv.Spec.Machine.
+Require riscv.Platform.Memory.
+Require Import riscv.Spec.PseudoInstructions.
+Require Import riscv.Proofs.EncodeBound.
+Require Import riscv.Proofs.DecodeEncode.
+Require Import riscv.Platform.Run.
+Require Import riscv.Utility.MkMachineWidth.
+Require Import riscv.Utility.Monads.
+Require Import riscv.Utility.runsToNonDet.
 Require Import coqutil.Datatypes.PropSet.
-Require Import riscv.MMIOTrace.
+Require Import riscv.Utility.MMIOTrace.
 
 Local Open Scope Z_scope.
 
@@ -29,8 +29,8 @@ Section Equiv.
   (* TODO not sure if we want to use ` or rather a parameter record *)
   Context {M: Type -> Type}.
   Context `{Pr: Primitives MMIOAction M}.
-  Context {RVS: RiscvState M word}.
-  Notation RiscvMachine := (RiscvMachine Register MMIOAction).
+  Context {RVS: riscv.Spec.Machine.RiscvMachine M word}.
+  Notation RiscvMachine := (riscv.Platform.RiscvMachine.RiscvMachine Register MMIOAction).
 
   Definition iset: InstructionSet := if width =? 32 then RV32IM else RV64IM.
 
